Sha3/ExamplesWithIntermediateValues.lean
@@ -1,0 +1,68 @@
+/- 
+See https://csrc.nist.gov/projects/cryptographic-standards-and-guidelines/example-values 
+-/
+import Sha3.Spec
+
+open Spec
+local instance: OfNat Bool 0 where ofNat := false
+local instance: OfNat Bool 1 where ofNat := true
+
+-- SHA3
+-- Message 0 bytes
+#eval BitString.dump (spacing? := false) <| SHA3_224 #[]
+#eval BitString.dump (spacing? := false) <| SHA3_256 #[]
+#eval BitString.dump (spacing? := false) <| SHA3_384 #[]
+#eval BitString.dump (spacing? := false) <| SHA3_512 #[]
+-- Message 30 bytes
+#eval BitString.dump (spacing? := false) <|
+  SHA3_224 <| Array.mk <| [1, 1, 0, 0, 1, 0, 1, 0, 0, 0, 0, 1, 1, 0, 1, 0, 1, 1, 0, 1, 1, 1, 1, 0, 1, 0, 0, 1, 1, 0]
+#eval BitString.dump (spacing? := false) <|
+  SHA3_256 <| Array.mk <| [1, 1, 0, 0, 1, 0, 1, 0, 0, 0, 0, 1, 1, 0, 1, 0, 1, 1, 0, 1, 1, 1, 1, 0, 1, 0, 0, 1, 1, 0]
+#eval BitString.dump (spacing? := false) <|
+  SHA3_384 <| Array.mk <| [1, 1, 0, 0, 1, 0, 1, 0, 0, 0, 0, 1, 1, 0, 1, 0, 1, 1, 0, 1, 1, 1, 1, 0, 1, 0, 0, 1, 1, 0]
+#eval BitString.dump (spacing? := false) <|
+  SHA3_512 <| Array.mk <| [1, 1, 0, 0, 1, 0, 1, 0, 0, 0, 0, 1, 1, 0, 1, 0, 1, 1, 0, 1, 1, 1, 1, 0, 1, 0, 0, 1, 1, 0]
+-- Message 1600 bytes
+#eval BitString.dump (spacing? := false) <|
+  SHA3_224 <| Array.mk <| (List.replicate 200 [1,1,0,0, 0,1,0,1] |>.flatten)
+#eval BitString.dump (spacing? := false) <|
+  SHA3_256 <| Array.mk <| (List.replicate 200 [1,1,0,0, 0,1,0,1] |>.flatten)
+#eval BitString.dump (spacing? := false) <|
+  SHA3_384 <| Array.mk <| (List.replicate 200 [1,1,0,0, 0,1,0,1] |>.flatten)
+#eval BitString.dump (spacing? := false) <|
+  SHA3_512 <| Array.mk <| (List.replicate 200 [1,1,0,0, 0,1,0,1] |>.flatten)
+-- Message 1605 bytes
+#eval BitString.dump (spacing? := false) <|
+  SHA3_224 <| Array.mk <| (List.replicate 200 [1,1,0,0, 0,1,0,1] |>.flatten) ++ [1,1,0,0, 0]
+#eval BitString.dump (spacing? := false) <|
+  SHA3_256 <| Array.mk <| (List.replicate 200 [1,1,0,0, 0,1,0,1] |>.flatten) ++ [1,1,0,0, 0]
+#eval BitString.dump (spacing? := false) <|
+  SHA3_384 <| Array.mk <| (List.replicate 200 [1,1,0,0, 0,1,0,1] |>.flatten) ++ [1,1,0,0, 0]
+#eval BitString.dump (spacing? := false) <|
+  SHA3_512 <| Array.mk <| (List.replicate 200 [1,1,0,0, 0,1,0,1] |>.flatten) ++ [1,1,0,0, 0]
+-- Message 1630 bytes
+#eval BitString.dump (spacing? := false) <|
+  SHA3_224 <| Array.mk <| (List.replicate 203 [1,1,0,0, 0,1,0,1] |>.flatten) ++ [1,1,0,0, 0,1]
+#eval BitString.dump (spacing? := false) <|
+  SHA3_256 <| Array.mk <| (List.replicate 200 [1,1,0,0, 0,1,0,1] |>.flatten) ++ [1,1,0,0, 0,1]
+#eval BitString.dump (spacing? := false) <|
+  SHA3_384 <| Array.mk <| (List.replicate 200 [1,1,0,0, 0,1,0,1] |>.flatten) ++ [1,1,0,0, 0,1]
+#eval BitString.dump (spacing? := false) <|
+  SHA3_512 <| Array.mk <| (List.replicate 200 [1,1,0,0, 0,1,0,1] |>.flatten) ++ [1,1,0,0, 0,1]
+
+
+-- Shake truncation
+-- Output length = 4096
+#eval BitString.dump (spacing? := true) <| SHAKE128 (d := 4096) #[]
+-- Output length = 4095
+#eval BitString.dump (spacing? := true) <| SHAKE128 (d := 4095) #[]
+-- Output length = 4094
+#eval BitString.dump (spacing? := true) <| SHAKE128 (d := 4094) #[]
+-- Output length = 4093
+#eval BitString.dump (spacing? := true) <| SHAKE128 (d := 4093) #[]
+-- Output length = 4092 -- TODO
+#eval BitString.dump (spacing? := true) <| SHAKE128 (d := 4092) #[]
+-- Output length = 4091 -- TODO
+#eval BitString.dump (spacing? := true) <| SHAKE128 (d := 4091) #[]
+-- Output length = 4090 -- TODO
+#eval BitString.dump (spacing? := true) <| SHAKE128 (d := 4090) #[]
