Sha3/Utils.lean
@@ -1,0 +1,79 @@
+/- private def Vector.xor(v: Vector Bool n): Bool := v.foldl (·^^·) false -/
+/- private def Vector.modify(v: Vector α n)(i: Fin n)(modif: α → α) : Vector α n := -/
+/-   ⟨v.toArray.modify i modif, by simp only [Array.size_modify, size_toArray] ⟩ -/
+def Vector.adjust(acc: Vector α n)(len: Nat)(fill: α): Vector α len := 
+  let res := acc.toArray.take len ++ (Array.mkArray (len - n) fill)
+  ⟨res, by 
+    simp [res]
+    cases h: decide (len > n) <;> simp at *
+    · simp [Nat.min_eq_left h]
+      exact Nat.sub_eq_zero_iff_le.mpr h
+    · simp [Nat.min_eq_right (Nat.le_of_lt h)]
+      simp [←Nat.add_sub_assoc (Nat.le_of_lt h) n]
+      simp [Nat.add_sub_cancel_left]
+    ⟩
+
+def Array.chunks(k: Nat)(arr: Array α): Array (Vector α k) :=
+  assert! arr.size % k == 0
+  if h: arr.size < k ∨ k = 0 then 
+    #[]
+  else
+    #[⟨arr.extract (stop := k), by simp_all [Nat.min_eq_left]⟩] ++ (arr.extract (start := k)).chunks k
+termination_by arr.size
+
+def Array.chunks' (k: Nat)(arr: Array α): Array (Array α) := 
+  if arr.size = 0 ∨ k = 0 then #[] else #[arr.take k] ++ (arr.drop k |>.chunks' k)
+termination_by arr.size
+
+def String.zfill(s: String)(len: Nat) := List.asString <|
+  (List.replicate (len - s.length) '0') ++ (s.take len).toList
+
+
+def UInt8.toBitString(u: UInt8): Vector Bool 8 :=
+  let bv := u.toBitVec
+  #v[ (bv >>> 0) % 2 == 1,
+      (bv >>> 1) % 2 == 1,
+      (bv >>> 2) % 2 == 1,
+      (bv >>> 3) % 2 == 1,
+      (bv >>> 4) % 2 == 1,
+      (bv >>> 5) % 2 == 1,
+      (bv >>> 6) % 2 == 1,
+      (bv >>> 7) % 2 == 1 ]
+
+/- private def Vector.ofArray(arr: Array α): Vector α arr.size := ⟨arr, rfl⟩ -/
+def ByteArray.toBitArray(arr: ByteArray): Array Bool :=
+  arr.data
+    |>.map (·.toBitString.toArray)
+    |>.flatten
+def String.toUTF8Bits := ByteArray.toBitArray ∘ toUTF8
+
+def Utils.toNat(S: Vector Bool n): Nat := S.mapIdx (2^· * if · then 1 else 0) |>.sum
+def Utils.toHex (S: Vector Bool n): String := S 
+  |> Utils.toNat
+  |>.toDigits (base := 16) |>.asString
+open Std.Format in 
+def Utils.dump (S: Vector Bool n)(spacing? : Bool := false): Std.Format := --S.toNat.toDigits (base := 16) |>.asString
+    let width := 8
+    let singleSpace? := if spacing? then text " " else nil
+    let lineBreak? := if spacing? then align false else nil
+    let final := S.adjust (width * ((S.size + width-1)/width)) false
+      |>.chunks width
+      |>.map (fun lane => Utils.toHex lane |>.zfill (width/4))
+      |>.toList
+      |> "".intercalate
+      |>.zfill ((S.size + 3) / 4)
+    let formatted := Array.mk final.toList
+      |>.chunks' 16
+      |>.map (·.chunks' 2 
+        |>.map (fun v => text  <| v.toList.asString) 
+        |>.toList 
+        |> singleSpace?.joinSep
+        |> group)
+      |>.chunks' 2
+      |>.map (·.toList |> singleSpace?.joinSep)
+      |>.toList
+      |> lineBreak?.joinSep
+    if spacing? then 
+      nest 8 <| lineBreak? ++ formatted
+    else
+      formatted
